checkpoint gardening

Order/Logic.lean
@@ -1,9 +1,11 @@
+import Order.Lib
+
 /-
 # Separation Logic
 -/
 
 /-
-Syntax of a generic separation logic
+## Syntax
 -/
 inductive L (B : Type)
 | base (b  : B) : L B
@@ -23,140 +25,661 @@ def L.top : L B := L.neg L.bot
 
 open L
 
-/--
-Shallow embedding of Hilbert-style IP proof system
 
-Used to derive generic rules
--/
-class IP (R : L B -> Prop) where
-  mp    : R φ -> R (imp φ ψ) -> R ψ
-  imp1  : R <| imp φ <| imp ψ φ
-  imp2  : R <| imp (imp φ (imp ψ χ)) <| imp (imp φ ψ) <| imp φ χ
-  andI  : R <| imp φ <| imp ψ (and φ ψ)
-  andE1 : R <| imp (and φ ψ) φ
-  andE2 : R <| imp (and φ ψ) ψ
-  orI1  : R <| imp φ (or φ ψ)
-  orI2  : R <| imp ψ (or φ ψ)
-  orE   : R <| imp (imp φ χ) <| imp (imp ψ χ) <| imp (or φ ψ) χ
-  botE  : R <| imp bot φ
+
+
 
 
 /-
-Shallow embedding of optional axioms
+## Separation Algebras
 -/
 
-class WEM (R : L B -> Prop) extends IP R where
-  wem : R <| or (neg φ) (neg (neg φ))
-
-class GD (R : L B -> Prop) extends IP R where
-  gd : R <| or (imp φ ψ) (imp ψ φ)
-
-class EM (R : L B -> Prop) extends IP R where
-  em : R <| or φ (neg φ)
-
-/--
-Shallow embedding of SL axioms
--/
-class SL (R : L B -> Prop) extends IP R where
-  scomm  : R <| imp (sep φ ψ) (sep ψ φ)
-  sA1    : (R <| imp (sep φ ψ) χ) -> (R <| imp φ (wand ψ χ))
-  sA2    : (R <| imp φ (wand ψ χ)) -> (R <| imp (sep φ ψ) χ)
-  semp   : R <| iff (sep φ emp) φ
-  sassoc : R <| imp (sep (sep φ ψ) χ) <| (sep φ (sep ψ χ))
-  smono  : R (imp φ1 ψ1) -> R (imp φ2 ψ2) -> R (imp (sep φ1 φ2) (sep ψ1 ψ2))
-
-/-
-Shallow embedding of optional SL actioms
--/
-
-class GC (R : L B -> Prop) extends SL R where
-  starE : R <| imp (sep φ ψ) φ
-
-class EE (R : L B -> Prop) extends SL R where
-  eE : R <| imp (and emp (sep φ ψ)) φ
-
-class EDup (R : L B -> Prop) extends SL R where
-  eDup : R <| imp (and emp φ) <| (sep φ φ)
-
-class MallocFree (R : L B -> Prop) extends EE R, EDup R
-
-/-
-Derived laws
--/
-/-
-def wandE1 [IP R] [SL R] : R <| imp (sep (wand ϕ ψ) ϕ) ψ := by sorry
-
-def or_sep_iff [IP R] [SL R] : R <| iff (sep (or ϕ ψ) χ) (or (sep ϕ ψ) (sep ϕ χ)) := sorry
-
-def and_sep_iff [IP R] [SL R] : R <| iff (sep (and ϕ ψ) χ) (and (sep ϕ ψ) (sep ϕ χ)) := sorry
--/
-
-
-/-
-Separation Algebras
--/
+/-- A type equipped with separating conjunction -/
 class SepC (M : Type) where
   sepC : M -> M -> M
 
 infixl:65 " ∗ " => SepC.sepC
 
-class SA (M : Type) [SepC M] where
-  sepC_assoc : ∀ m0 m1 m2 : M, (m0 ∗ m1) ∗ m2 = m0 ∗ (m1 ∗ m2)
-  sepC_comm : ∀ m0 m1 : M, m0 ∗ m1 = m1 ∗ m0
+/-- A sepration algebra over M -/
+class SeparationAlgebra (M : Type) [S : SepC M] extends (Std.Associative S.sepC), (Std.Commutative S.sepC)
+
 
 
 /-
-Semantics
+## Kripke Models
 -/
+
+/-- Validity of base propositions B in a sepration algebra M -/
 class Kripke.AtomicInterp (M B : Type) where
   ainterp : M -> B -> Prop
 
+/-- A type equipped with an order -/
 class Kripke.Ord (M : Type) where
   kle : M -> M -> Prop
 infixl:65 " << " => Kripke.Ord.kle
 
-def is_increasing [Kripke.Ord M] [SepC M] (e : M) : Prop :=
+/-- An element is increasing -/
+def Kripke.is_increasing [Ord M] [SepC M] (e : M) : Prop :=
   ∀ m n : M, e ∗ m = n -> m << n
 
-class Kripke.Structure (M : Type) extends Kripke.Ord M where
-  kle_refl : ∀ m, kle m m
-  kle_trans : ∀ m1 m2 m3, kle m1 m2 -> kle m2 m3 -> kle m1 m3
+/-- A type equipped with a reflexive, transitive order -/
+class Kripke.Structure (M : Type) [O : Ord M] extends (Reflexive O.kle), (Transitive O.kle)
 
-class Kripke.Model (M B : Type) [Kripke.Structure M] [I : Kripke.AtomicInterp M B] where
-  kle_ainterp_mono : ∀ m n σ, m << n -> I.ainterp m σ -> I.ainterp n σ
+/-- A Kripke model is a Kripke structure where atomic propositions have monotnic denotation -/
+class Kripke.Model (M B : Type) [Ord M] [Structure M] extends AtomicInterp M B where
+  kle_ainterp_mono : ∀ m n σ, m << n -> ainterp m σ -> ainterp n σ
 
--- General interface for Kripke Semantics
-class Kripke.Semantics (M B : Type) [Kripke.Ord M] extends Kripke.AtomicInterp M B where
-  interp : M -> L B -> Prop
-  interp_base : interp m (L.base b) = Kripke.AtomicInterp.ainterp m b
-  interp_bot  : interp m L.bot = False
-  interp_and  : interp m (L.and l r) = (interp m l ∧ interp m r)
-  interp_or   : interp m (L.or l r) = (interp m l ∨ interp m r)
-  interp_imp  : interp m (L.imp l r) = ∀ m0, m << m0 -> interp m0 l -> interp m0 r
 
--- Interface for Kripke semantics with strong wand
-class Kripke.StrongWandSemantics (M B : Type) [Kripke.Ord M] [SepC M] (S : Kripke.Semantics M B) where
-  interp_wand : S.interp m (L.wand l r) = ∀ m0 m1 m2 : M, m << m0 -> m0 ∗ m1 = m2 -> S.interp m1 l -> S.interp m2 r
 
--- Interface for Kripke semantics with strong sep
-class Kripke.StrongSepSemantics (M B : Type) [Kripke.Ord M] [SepC M] (S : Kripke.Semantics M B) where
-  interp_sep : S.interp m (L.sep l r) = ∃ m0 m1 m2 : M, m0 << m ∧ m1 ∗ m2 = m0 ∧ S.interp m1 l ∧ S.interp m2 r
 
--- Interface for Kripke semantics with weak wand
-class Kripke.WeakWandSemantics (M B : Type) [Kripke.Ord M] [SepC M] (S : Kripke.Semantics M B) where
-  interp_wand : S.interp m (L.wand l r) = ∀ m1 m2 : M, m ∗ m1 = m2 -> S.interp m1 l -> S.interp m2 r
 
--- Interface for Kripke semantics with weak sep
-class Kripke.WeakSepSemantics (M B : Type) [Kripke.Ord M] [SepC M] (S : Kripke.Semantics M B) where
-  interp_sep : S.interp m (L.sep l r) = ∃ m1 m2 : M, m1 ∗ m2 = m ∧ S.interp m1 l ∧ S.interp m2 r
-
--- Interface for Kripke semantics with emp
-class Kripke.EmpSemantics  (M B : Type) [Kripke.Ord M] [SepC M] (S : Kripke.Semantics M B) where
-  interp_emp  : S.interp m L.emp = is_increasing m
 
 /-
-Instances of Kripke semantics
+## Kripke Semantics
 -/
+
+/--
+A type has a Kripke semantics (an interpretation for (L B) terms under a world m)
+-/
+class Kripke.Semantics (M B : Type) [Ord M] [Structure M] extends Model M B where
+  interp : M -> L B -> Prop
+
+/-- A Kripke semantics obeys the base interpretation -/
+class Kripke.BaseSemantics (M B : Type) [Ord M] [Structure M] (S : Semantics M B) where
+  interp_base : S.interp m (L.base b) = S.ainterp m b
+  interp_bot  : S.interp m L.bot = False
+  interp_and  : S.interp m (L.and l r) = (S.interp m l ∧ S.interp m r)
+  interp_or   : S.interp m (L.or l r) = (S.interp m l ∨ S.interp m r)
+  interp_imp  : S.interp m (L.imp l r) = ∀ m0, m << m0 -> S.interp m0 l -> S.interp m0 r
+
+/-- A Kripke semantics obeys the strong wand interpretation -/
+class Kripke.StrongWandSemantics (M B : Type) [Ord M] [SepC M] [Structure M] (S : Semantics M B) where
+  interp_wand : S.interp m (L.wand l r) = ∀ m0 m1 m2 : M, m << m0 -> m0 ∗ m1 = m2 -> S.interp m1 l -> S.interp m2 r
+
+/-- A Kripke semantics obeys the strong separating conjunction interpretation -/
+class Kripke.StrongSepSemantics (M B : Type) [Ord M] [SepC M] [Structure M] (S : Semantics M B) where
+  interp_sep : S.interp m (L.sep l r) = ∃ m0 m1 m2 : M, m0 << m ∧ m1 ∗ m2 = m0 ∧ S.interp m1 l ∧ S.interp m2 r
+
+/-- A Kripke semantics obeys the strong weak wand interpretation -/
+class Kripke.WeakWandSemantics (M B : Type) [Ord M] [SepC M] [Structure M] (S : Semantics M B) where
+  interp_wand : S.interp m (L.wand l r) = ∀ m1 m2 : M, m ∗ m1 = m2 -> S.interp m1 l -> S.interp m2 r
+
+/-- A Kripke semantics obeys the strong weak separating conjunction interpretation -/
+class Kripke.WeakSepSemantics (M B : Type) [Ord M] [SepC M] [Structure M] (S : Semantics M B) where
+  interp_sep : S.interp m (L.sep l r) = ∃ m1 m2 : M, m1 ∗ m2 = m ∧ S.interp m1 l ∧ S.interp m2 r
+
+/-- A Kripke semantics obeys the interpretation of emp -/
+class Kripke.EmpSemantics (M B : Type) [Ord M] [SepC M] [Structure M] (S : Semantics M B) where
+  interp_emp  : S.interp m L.emp = is_increasing m
+
+/--
+A Flat Kripke semantics has weak wand and weak sep
+-/
+class Kripke.FlatSemantics (M B : Type) [Ord M] [SepC M] [Structure M] (S : Semantics M B) extends
+  BaseSemantics M B S,
+  WeakWandSemantics M B S,
+  WeakSepSemantics M B S,
+  EmpSemantics M B S
+
+
+
+/-
+## Variants of separation algebras
+-/
+
+
+/-- A separation algebra is upwards closed -/
+class UCSA (M : Type) [Kripke.Ord M] [SepC M] where
+  ucsa : ∀ {m1 m2 m n}, m1 ∗ m2 = m -> m << n -> ∃ (n1 n2 : M), n1 ∗ n2 = n ∧ m1 << n1 ∧ m2 << n2
+
+/-- A separation algebra is downwards closed -/
+class DCSA (M : Type) [Kripke.Ord M] [SepC M] where
+  dcsa : ∀ {m1 m2 m n1 n2}, m1 ∗ m2 = m -> n1 << m1 -> n2 << m2 -> ∃(n : M), n1 ∗ n2 = n ∧ n << m
+
+
+/-- m is a residue of n -/
+def residue [Kripke.Ord M] [SepC M] (m n : M) : Prop :=
+  ∃ n', m ∗ n' = n ∧ n << n'
+
+/-- All elements have an increasing residue -/
+class Unital (M : Type) [Kripke.Ord M] [SepC M] where
+  unital : ∀ m, ∃ unit : M, residue unit m ∧ Kripke.is_increasing unit
+
+
+/-- Variant of separation algebra where the base soundness proof applies -/
+class BaseAlgebra (M : Type) [Kripke.Ord M] [SepC M] extends
+  SeparationAlgebra M,
+  UCSA M,
+  DCSA M,
+  Unital M
+
+
+
+
+
+
+
+/-
+## Monotonicity
+-/
+
+/-- A term has monotonic denotation inside a Kripke semantics -/
+def Kripke.monotonic_denotation {M B : Type} [Ord M] [SepC M] [Structure M] (S : Kripke.Semantics M B) (e : L B) : Prop :=
+  ∀ {m n : M}, n << m -> S.interp n e -> S.interp m e
+
+
+section Mono
+
+variable {M : Type}
+variable [Kripke.Ord M] [SepC M] [Kripke.Structure M]
+variable (S : Kripke.Semantics M B)
+
+/-- Weak conjunction preserves monotonic denotation in a UCSA -/
+theorem Mono.weak_sep [W : Kripke.WeakSepSemantics M B S] [UCSA M] :
+    Kripke.monotonic_denotation S e1 ->
+    Kripke.monotonic_denotation S e2 ->
+    Kripke.monotonic_denotation S (L.sep e1 e2) := by
+  unfold Kripke.monotonic_denotation
+  simp [W.interp_sep]
+  intro M1 M2 m n Hnm m1 m2 Hm1m2 He1 He2
+  rcases (@UCSA.ucsa _ _ _ _ m1 m2 n m Hm1m2 Hnm) with ⟨ n1, n2, H1, H2, H3 ⟩
+  exists n1
+  exists n2
+  apply And.intro
+  · exact H1
+  apply And.intro
+  · apply M1 H2 He1
+  · apply M2 H3 He2
+
+/--
+Weak wand preserves monotonic denotation in a DCSA
+
+The left argument does not need to have monotonic denotation.
+-/
+theorem Mono.weak_wand [W : Kripke.WeakWandSemantics M B S] [DCSA M] :
+    Kripke.monotonic_denotation S e2 ->
+    Kripke.monotonic_denotation S (L.wand e1 e2) := by
+  unfold Kripke.monotonic_denotation
+  simp [W.interp_wand]
+  intro H2 m n Hmn H m1 He1
+  have Hm1 : m1 << m1 := by apply Reflexive.refl
+  rcases (@DCSA.dcsa _ _ _ _ m m1 (m ∗ m1) n m1 (by rfl) Hmn Hm1) with ⟨ n', Hn', Hn'mm1 ⟩
+  apply (H2 Hn'mm1)
+  rw [<- Hn']
+  apply H
+  apply He1
+
+
+/-- Strong conjunction has monotonic denotation -/
+theorem Mono.strong_sep [W : Kripke.StrongSepSemantics M B S] :
+    Kripke.monotonic_denotation S (L.sep e1 e2) := by
+  intro m n Hmn
+  simp [W.interp_sep]
+  intro x Hx x1 x2 Hx1x2 Hi1 Hi2
+  exists x
+  apply And.intro
+  · apply Transitive.trans Hx Hmn
+  exists x1
+  exists x2
+
+
+/-- Strong wand has monotonic denotation -/
+theorem Mono.strong_wand [W : Kripke.StrongWandSemantics M B S] :
+    Kripke.monotonic_denotation S (L.wand e1 e2) := by
+  intro m n Hmn
+  simp [W.interp_wand]
+  intro H m0 m1 Hm0m1 Hi1
+  apply H
+  · apply Transitive.trans Hmn Hm0m1
+  apply Hi1
+
+/-- Base semantics have monotonic denoatation -/
+theorem Mono.base [Kripke.BaseSemantics M B S] :
+    Kripke.monotonic_denotation S (L.base b) := by
+  unfold Kripke.monotonic_denotation
+  intro m n Hnm
+  simp [Kripke.BaseSemantics.interp_base]
+  intro H1
+  apply S.kle_ainterp_mono
+  · apply Hnm
+  · apply H1
+
+
+
+/-- bot has monotonic denotation -/
+theorem Mono.bot [Kripke.BaseSemantics M B S] :
+    Kripke.monotonic_denotation S L.bot := by
+  unfold Kripke.monotonic_denotation
+  simp [Kripke.BaseSemantics.interp_bot]
+
+
+
+/-- and preserves monotonic denotation -/
+theorem Mono.and [Kripke.BaseSemantics M B S] :
+    Kripke.monotonic_denotation S φ ->
+    Kripke.monotonic_denotation S ψ ->
+    Kripke.monotonic_denotation S (L.and φ ψ) := by
+  unfold Kripke.monotonic_denotation
+  simp [Kripke.BaseSemantics.interp_and]
+  intros Hm1 Hm2 ; intros
+  apply And.intro
+  · apply Hm1 <;> trivial
+  · apply Hm2 <;> trivial
+
+
+/-- or preserves monotonic denotation -/
+theorem Mono.or [Kripke.BaseSemantics M B S] :
+    Kripke.monotonic_denotation S φ ->
+    Kripke.monotonic_denotation S ψ ->
+    Kripke.monotonic_denotation S (L.or φ ψ) := by
+  unfold Kripke.monotonic_denotation
+  simp [Kripke.BaseSemantics.interp_or]
+  intro Hm1 Hm2 _ _ _ H
+  cases H
+  · left
+    apply Hm1 <;> trivial
+  · right
+    apply Hm2  <;> trivial
+
+/-- imp preserves monotonic denotation -/
+theorem Mono.imp  [Kripke.BaseSemantics M B S] :
+    Kripke.monotonic_denotation S (L.imp φ ψ) := by
+  unfold Kripke.monotonic_denotation
+  simp [Kripke.BaseSemantics.interp_imp ]
+  intro m n Hmn H m1 Hm1 H2
+  apply H
+  · apply Transitive.trans Hmn Hm1
+  trivial
+
+
+/-- emp has monotonic denotation in any downwards-closed semantics -/
+theorem Mono.emp_dcsa [Kripke.EmpSemantics M B S] [DCSA M] :
+    Kripke.monotonic_denotation S L.emp := by
+  unfold Kripke.monotonic_denotation
+  simp [Kripke.EmpSemantics.interp_emp]
+  intro m n Hnm
+  simp [Kripke.is_increasing]
+  intro h1 m2
+  rcases (DCSA.dcsa (by rfl) Hnm Reflexive.refl) with ⟨ n', Hn', H'n' ⟩
+  apply Transitive.trans _ H'n'
+  rw [<- Hn']
+  apply h1
+
+
+/--
+Monotonicity of the flat semantics in a base model (Base algebra with flat semantics )
+-/
+theorem BaseModel.mono [BaseAlgebra M] [Kripke.FlatSemantics M B S] :
+    ∀ {e}, Kripke.monotonic_denotation S e := by
+  intro e
+  induction e
+  · apply Mono.base
+  · apply Mono.bot
+  · apply Mono.and <;> trivial
+  · apply Mono.or <;> trivial
+  · apply Mono.imp
+  · apply Mono.emp_dcsa
+  · apply Mono.weak_sep <;> trivial
+  · apply Mono.weak_wand <;> trivial
+
+end Mono
+
+
+
+
+
+/-
+## Soudness for the base model
+-/
+
+section soundness
+
+variable {M B : Type}
+variable [Kripke.Ord M] [Kripke.Structure M] [SepC M]
+variable (S : Kripke.Semantics M B)
+variable [BaseAlgebra M]
+variable [Kripke.FlatSemantics M B S]
+
+theorem Soundness.imp1 {φ ψ : L B} :
+    ∀ m : M, S.interp m <| imp φ <| imp ψ φ := by
+  intro m
+  rw [Kripke.BaseSemantics.interp_imp]
+  intro m0 _ Hφ
+  rw [Kripke.BaseSemantics.interp_imp]
+  intro m1 Hm1 _
+  apply BaseModel.mono
+  · apply Hm1
+  apply Hφ
+
+omit [BaseAlgebra M] in
+theorem Soundness.imp2 {φ ψ : L B} :
+    ∀ m : M, S.interp m <| imp (imp φ (imp ψ χ)) <| imp (imp φ ψ) <| imp φ χ := by
+  intro m
+  simp [Kripke.BaseSemantics.interp_imp]
+  intro m1 _ H m2 Hm2 H3 m4 Hm4 Hm4φ
+  apply (H _ ?G1 Hm4φ m4 ?G2)
+  case G1 => apply Transitive.trans Hm2 Hm4
+  case G2 => apply Reflexive.refl
+  apply (H3 _ Hm4 Hm4φ)
+
+theorem Soundness.andI {φ ψ : L B} :
+    ∀ m : M, S.interp m <| imp φ <| imp ψ (and φ ψ) := by
+  simp [Kripke.BaseSemantics.interp_imp, Kripke.BaseSemantics.interp_and]
+  intro m0 m1 _ Hφ m3 Hm1m3 Hψ
+  apply And.intro
+  · apply BaseModel.mono _ Hm1m3
+    trivial
+  · trivial
+
+omit [BaseAlgebra M] in
+theorem Soundness.andE1 {φ ψ : L B} :
+    ∀ m : M, S.interp m <| imp (and φ ψ) φ := by
+  simp [Kripke.BaseSemantics.interp_imp, Kripke.BaseSemantics.interp_and]
+  intros
+  trivial
+
+omit [BaseAlgebra M] in
+theorem Soundness.andE2 {φ ψ : L B} :
+    ∀ m : M, S.interp m <| imp (and φ ψ) ψ := by
+  simp [Kripke.BaseSemantics.interp_imp, Kripke.BaseSemantics.interp_and]
+
+omit [BaseAlgebra M] in
+theorem Soundness.orI1 {φ ψ : L B} :
+    ∀ m : M, S.interp m <| imp φ (or φ ψ) := by
+  simp [Kripke.BaseSemantics.interp_imp, Kripke.BaseSemantics.interp_or]
+  intros
+  left
+  trivial
+
+omit [BaseAlgebra M] in
+theorem Soundness.orI2 {φ ψ : L B} :
+    ∀ m : M, S.interp m <| imp ψ (or φ ψ) := by
+  simp [Kripke.BaseSemantics.interp_imp, Kripke.BaseSemantics.interp_or]
+  intros
+  right
+  trivial
+
+omit [BaseAlgebra M] in
+theorem Soundness.orE {φ ψ : L B} :
+    ∀ m : M, S.interp m <| imp (imp φ χ) <| imp (imp ψ χ) <| imp (or φ ψ) χ := by
+  simp [Kripke.BaseSemantics.interp_imp, Kripke.BaseSemantics.interp_or]
+  intro m0 m1 _ H1 m2 m1m2 H2 m3 m2m3 H3
+  cases H3
+  · apply H1
+    · exact Transitive.trans m1m2 m2m3
+    · trivial
+  · apply H2
+    · exact m2m3
+    · trivial
+
+omit [BaseAlgebra M] in
+theorem Soundness.botE {φ : L B} :
+    ∀ m : M, S.interp m <| imp bot φ := by
+  simp [Kripke.BaseSemantics.interp_imp, Kripke.BaseSemantics.interp_bot]
+
+omit [BaseAlgebra M] in
+theorem Soundness.mp {φ ψ : L B} :
+    ∀ m : M, S.interp m φ -> S.interp m (imp φ ψ) -> S.interp m ψ := by
+  simp [Kripke.BaseSemantics.interp_imp]
+  intro m Hφ H
+  apply H
+  · apply Reflexive.refl
+  · trivial
+
+theorem Soundness.scomm {φ : L B} :
+    ∀ m : M, S.interp m <| imp (sep φ ψ) (sep ψ φ) := by
+  simp [Kripke.BaseSemantics.interp_imp]
+  intro m0 m1 _
+  simp [Kripke.WeakSepSemantics.interp_sep]
+  intro m2 m3 m2m3 Hφ Hψ
+  exists m3
+  exists m2
+  apply And.intro
+  ·
+    sorry
+    -- rw [SeparationAlgebra.sepC_comm]
+    -- trivial
+  apply And.intro
+  · trivial
+  · trivial
+
+/-
+theorem Soundness.sA1 {φ : L B}
+    [Kripke.Structure M] (S : Kripke.Semantics M B) [Kripke.Model M B] [SoundIPModel M] [FlatSemantics M B S] [SeparationAlgebra M] :
+    (∀ m : M, (S.interp m <| imp (sep φ ψ) χ)) -> (∀ m : M, (S.interp m <| imp φ (wand ψ χ))) := by
+  simp [Kripke.Semantics.interp_imp, Kripke.WeakSepSemantics.interp_sep, Kripke.WeakWandSemantics.interp_wand]
+  intro H m1 m2 _ Hφ m3 Hψ
+  apply H (m2 ∗ m3) (m2 ∗ m3) (Kripke.Structure.kle_refl (m2 ∗ m3)) m2 m3 (by rfl) Hφ Hψ
+
+theorem Soundness.sA2 {φ : L B}
+    [Kripke.Structure M] (S : Kripke.Semantics M B) [Kripke.Model M B] [SoundIPModel M] [FlatSemantics M B S] [SeparationAlgebra M] :
+    (∀ m : M, (S.interp m <| imp φ (wand ψ χ))) -> (∀ m : M, S.interp m <| imp (sep φ ψ) χ) := by
+  simp [Kripke.Semantics.interp_imp, Kripke.WeakSepSemantics.interp_sep, Kripke.WeakWandSemantics.interp_wand]
+  intro H m1 m2 m0m1 m3 m4 m3m42 Hφ Hψ
+  subst m3m42
+  apply H m3 m3 (Kripke.Structure.kle_refl m3) Hφ m4 Hψ
+
+theorem Soundness.semp {φ : L B}
+    [Kripke.Structure M] (S : Kripke.Semantics M B) [Kripke.Model M B] [SoundIPModel M] [FlatSemantics M B S] [SeparationAlgebra M] :
+    ∀ m : M, S.interp m <| iff (sep φ emp) φ := by
+  unfold L.iff
+  simp [Kripke.Semantics.interp_and, Kripke.Semantics.interp_imp, Kripke.WeakSepSemantics.interp_sep, Kripke.EmpSemantics.interp_emp]
+  intro m0
+  apply And.intro
+  · intro m1 _ m2 m3 m231 Hφ HI
+    apply SoundIPModel.mono _ _ _ _ _ m2 ?G2 ?G3
+    · apply HI
+      sorry
+      -- rw [SA.sepC_comm]
+      -- trivial
+    · trivial
+  · intro m1 _ Hφ
+    rcases (Unital.unital m1) with ⟨ m1u, ⟨ m1r, Em1, Hm1r ⟩, Hu ⟩
+    exists m1r
+    exists m1u
+    apply And.intro
+    · sorry
+      -- rw [SA.sepC_comm]
+      -- trivial
+    apply And.intro
+    · apply SoundIPModel.mono _ _ _ _ _ m1 Hm1r Hφ
+    · trivial
+
+theorem Soundness.sassoc {φ : L B}
+    [Kripke.Structure M] (S : Kripke.Semantics M B) [Kripke.Model M B] [SoundIPModel M] [FlatSemantics M B S] [SeparationAlgebra M] :
+    ∀ m : M, S.interp m <| imp (sep (sep φ ψ) χ) <| (sep φ (sep ψ χ)) := by
+  simp [Kripke.Semantics.interp_imp, Kripke.WeakSepSemantics.interp_sep]
+  intro m0 m1 m0m1 m2 m3 m231 m4 m5 m452
+  subst m231
+  subst m452
+  intro Hφ Hψ Hχ
+  exists m4
+  exists (m5 ∗ m3)
+  apply And.intro
+  ·
+    sorry
+    -- apply Eq.symm (SA.sepC_assoc m4 m5 m3)
+  apply And.intro
+  · trivial
+  exists m5
+  exists m3
+
+theorem Soundness.smono
+    [Kripke.Structure M] (S : Kripke.Semantics M B) [Kripke.Model M B] [SoundIPModel M] [FlatSemantics M B S] [SeparationAlgebra M] :
+    (∀ m : M, (S.interp m <| imp φ1 ψ1)) -> (∀ m : M, S.interp m <| imp φ2 ψ2) -> (∀ m : M, S.interp m <| imp (sep φ1 φ2) (sep ψ1 ψ2)) := by
+  simp [Kripke.Semantics.interp_imp, Kripke.WeakSepSemantics.interp_sep]
+  intro H1 H2 m0 m1 m01 m2 m3 m231 Hp1 Hp2
+  subst m231
+  exists m2
+  exists m3
+  apply And.intro
+  · rfl
+  apply And.intro
+  · apply H1 m2 m2 (Kripke.Structure.kle_refl m2) Hp1
+  · apply H2 m3 m3 (Kripke.Structure.kle_refl m3) Hp2
+
+-/
+end soundness
+
+/-
+/-
+Soundness for the extensions
+-/
+
+
+
+/-
+Soundness for the basic IP+SL system (removed base props)
+-/
+
+inductive IPSL_deriv {B : Type} : L B -> Prop
+| mp     : IPSL_deriv φ -> IPSL_deriv (imp φ ψ) -> IPSL_deriv ψ
+| imp1   : IPSL_deriv <| imp φ <| imp ψ φ
+| imp2   : IPSL_deriv <| imp (imp φ (imp ψ χ)) <| imp (imp φ ψ) <| imp φ χ
+| andI   : IPSL_deriv <| imp φ <| imp ψ (and φ ψ)
+| andE1  : IPSL_deriv <| imp (and φ ψ) φ
+| andE2  : IPSL_deriv <| imp (and φ ψ) ψ
+| orI1   : IPSL_deriv <| imp φ (or φ ψ)
+| orI2   : IPSL_deriv <| imp ψ (or φ ψ)
+| orE    : IPSL_deriv <| imp (imp φ χ) <| imp (imp ψ χ) <| imp (or φ ψ) χ
+| botE   : IPSL_deriv <| imp bot φ
+| scomm  : IPSL_deriv <| imp (sep φ ψ) (sep ψ φ)
+| sA1    : IPSL_deriv (imp (sep φ ψ) χ) -> IPSL_deriv (imp φ (wand ψ χ))
+| sA2    : IPSL_deriv (imp φ (wand ψ χ)) -> IPSL_deriv (imp (sep φ ψ) χ)
+| semp   : IPSL_deriv (iff (sep φ emp) φ)
+| sassoc : IPSL_deriv (imp (sep (sep φ ψ) χ) <| (sep φ (sep ψ χ)))
+| smono  : IPSL_deriv (imp φ1 ψ1) -> IPSL_deriv (imp φ2 ψ2) -> IPSL_deriv (imp (sep φ1 φ2) (sep ψ1 ψ2))
+
+/-
+instance ISPL_deriv_IP_inst {B} : IP (@IPSL_deriv B) where
+mp     := IPSL_deriv.mp
+imp1   := IPSL_deriv.imp1
+imp2   := IPSL_deriv.imp2
+andI   := IPSL_deriv.andI
+andE1  := IPSL_deriv.andE1
+andE2  := IPSL_deriv.andE2
+orI1   := IPSL_deriv.orI1
+orI2   := IPSL_deriv.orI2
+orE    := IPSL_deriv.orE
+botE   := IPSL_deriv.botE
+
+instance ISPL_deriv_SL_inst {B} : SL (@IPSL_deriv B) where
+scomm  := IPSL_deriv.scomm
+sA1    := IPSL_deriv.sA1
+sA2    := IPSL_deriv.sA2
+semp   := IPSL_deriv.semp
+sassoc := IPSL_deriv.sassoc
+smono  := IPSL_deriv.smono
+-/
+
+
+theorem IPSL_kripke_soundness {B : Type} [Kripke.Structure M] (S : Kripke.Semantics M B) [Kripke.Model M B] [SoundIPModel M] [FlatSemantics M B S] :
+    ∀ φ : L B, IPSL_deriv φ -> ∀ m, S.interp m φ := by
+  intro φ H
+  induction H
+  · rename_i _ _ _ _ IH1 IH2
+    intro m
+    apply Soundness.mp
+    · apply IH1
+    · apply IH2
+  · apply Soundness.imp1
+  · apply Soundness.imp2
+  · apply Soundness.andI
+  · apply Soundness.andE1
+  · apply Soundness.andE2
+  · apply Soundness.orI1
+  · apply Soundness.orI2
+  · apply Soundness.orE
+  · apply Soundness.botE
+  · apply Soundness.scomm
+  · apply Soundness.sA1
+    trivial
+  · apply Soundness.sA2
+    trivial
+  · apply Soundness.semp
+  · apply Soundness.sassoc
+  · apply Soundness.smono
+    · trivial
+    · trivial
+
+
+
+
+
+/-
+section sound_model
+
+-- Now if we can exhibit _some_ Kripke model with the above requirements, to prove the IPSL system is sound
+
+instance discrete_order {T : Type} : Kripke.Ord T where
+  kle := Eq
+
+instance discrete_structure {T : Type} : Kripke.Structure T where
+  kle_refl _ := by rfl
+  kle_trans := by
+    unfold Kripke.Ord.kle
+    unfold discrete_order
+    simp
+
+instance discrete_triv_ainterp {T1 T2: Type} : Kripke.AtomicInterp T1 T2 where
+  ainterp _ _ := True
+
+instance sepC_unit : SepC Unit where
+  sepC _ _ := PUnit.unit
+
+-- #check
+instance discrete_model {T : Type} : Kripke.Model T Unit  where
+  kle_ainterp_mono _ _ _ H _ := by rw [<- H]; trivial
+
+
+
+instance unit_SA : SeparationAlgebra Unit where
+  sepC_assoc := by sorry
+  sepC_comm  := by sorry
+
+
+instance unit_UCSA : UCSA Unit where
+  ucsa := by simp [Kripke.Ord.kle]
+
+instance unit_DCSA : DCSA Unit where
+  dcsa := by simp [Kripke.Ord.kle]
+
+instance unit_Unital : Unital Unit where
+  unital := by simp [residue, is_increasing, Kripke.Ord.kle]
+
+instance unit_SoundIPModel : SoundIPModel Unit where
+  inst_sepC := sepC_unit
+  inst_SA := unit_SA
+  inst_ucsa := unit_UCSA
+  inst_dcsa := unit_DCSA
+  inst_unital := unit_Unital
+
+
+def UnitSemantics : Kripke.Semantics Unit Unit := (@flat_semantics Unit Unit _ _ _)
+
+instance unit_empSemantics : Kripke.EmpSemantics Unit Unit UnitSemantics where
+  interp_emp := by simp [Kripke.Semantics.interp, UnitSemantics, flat_semantics]
+
+instance unit_weakWand : Kripke.WeakWandSemantics Unit Unit UnitSemantics where
+  interp_wand := by simp [Kripke.Semantics.interp, UnitSemantics, flat_semantics]
+
+instance unit_weakSep : Kripke.WeakSepSemantics Unit Unit UnitSemantics where
+  interp_sep := by simp [Kripke.Semantics.interp, UnitSemantics, flat_semantics]
+
+instance unit_flatSemantics : FlatSemantics Unit _ UnitSemantics where
+  inst_EmpSemantics := unit_empSemantics
+  inst_WeakWandSemantics := unit_weakWand
+  inst_WeakSepSemantics := unit_weakSep
+
+-- theorem IPSL_unit_soundness : @IPSL_deriv Unit bot -> False := by
+--   intro K
+--   have X := @IPSL_kripke_soundness Unit Unit _ UnitSemantics discrete_model unit_SoundIPModel _ bot K PUnit.unit
+--   simp [Kripke.Semantics.interp, UnitSemantics, flat_semantics] at X
+
+end sound_model
+-/
+-/
+/-
 
 /--
 Flat semantics: both sep and wand are weak
@@ -250,541 +773,13 @@ instance downwards_weak_wand [Kripke.Structure M] [Kripke.AtomicInterp M B] [Sep
 instance downwards_strong_sep [Kripke.Structure M] [Kripke.AtomicInterp M B] [SepC M] : Kripke.StrongSepSemantics M B downwards_semantics where
   interp_sep := by simp [Kripke.Semantics.interp]
 
-/--
-Monotonic denotations
+
 -/
-def Kripke.monotonic_denotation [Kripke.Ord M] (S : Kripke.Semantics M B) (e : L B) : Prop :=
-  ∀ m n : M, n << m -> S.interp n e -> S.interp m e
 
-class UCSA (M : Type) [Kripke.Ord M] [SepC M] where
-  ucsa : ∀ m1 m2 m n, m1 ∗ m2 = m -> m << n -> ∃ (n1 n2 : M), n1 ∗ n2 = n ∧ m1 << n1 ∧ m2 << n2
-
-class DCSA (M : Type) [Kripke.Ord M] [SepC M] where
-  dcsa : ∀ m1 m2 m n1 n2, m1 ∗ m2 = m -> n1 << m1 -> n2 << m2 -> ∃(n : M), n1 ∗ n2 = n ∧ n << m
-
-theorem Mono.weak_sep [Kripke.Ord M] [SepC M] (S : Kripke.Semantics M B) [W : Kripke.WeakSepSemantics M B S] [UCSA M] :
-    Kripke.monotonic_denotation S e1 ->
-    Kripke.monotonic_denotation S e2 ->
-    Kripke.monotonic_denotation S (L.sep e1 e2) := by
-  unfold Kripke.monotonic_denotation
-  simp [W.interp_sep]
-  intro M1 M2 m n Hnm m1 m2 Hm1m2 He1 He2
-  rcases (@UCSA.ucsa _ _ _ _ m1 m2 n m Hm1m2 Hnm) with ⟨ n1, n2, H1, H2, H3 ⟩
-  exists n1
-  exists n2
-  apply And.intro
-  · exact H1
-  apply And.intro
-  · exact M1 n1 m1 H2 He1
-  · exact M2 n2 m2 H3 He2
-
-theorem Mono.weak_wand [Kripke.Structure M] [SepC M] (S : Kripke.Semantics M B) [W : Kripke.WeakWandSemantics M B S] [DCSA M] :
-    -- Kripke.monotonic_denotation S e1 ->
-    Kripke.monotonic_denotation S e2 ->
-    Kripke.monotonic_denotation S (L.wand e1 e2) := by
-  unfold Kripke.monotonic_denotation
-  simp [W.interp_wand]
-  intro H2 m n Hmn H m1 He1
-  have Hm1 : m1 << m1 := by apply Kripke.Structure.kle_refl
-  rcases (@DCSA.dcsa _ _ _ _ m m1 (m ∗ m1) n m1 (by rfl) Hmn Hm1) with ⟨ n', Hn', Hn'mm1 ⟩
-  apply (H2 (m ∗ m1) n' Hn'mm1)
-  rw [<- Hn']
-  apply H
-  apply He1
-
-theorem Mono.strong_sep [Kripke.Structure M] [SepC M] (S : Kripke.Semantics M B) [W : Kripke.StrongSepSemantics M B S] :
-    -- Kripke.monotonic_denotation S e1 ->
-    -- Kripke.monotonic_denotation S e2 ->
-    Kripke.monotonic_denotation S (L.sep e1 e2) := by
-  intro m n Hmn
-  simp [W.interp_sep]
-  intro x Hx x1 x2 Hx1x2 Hi1 Hi2
-  exists x
-  apply And.intro
-  · exact Kripke.Structure.kle_trans x n m Hx Hmn
-  exists x1
-  exists x2
-
-theorem Mono.strong_wand [Kripke.Structure M] [SepC M] (S : Kripke.Semantics M B) [W : Kripke.StrongWandSemantics M B S] :
-    -- Kripke.monotonic_denotation S e1 ->
-    -- Kripke.monotonic_denotation S e2 ->
-    Kripke.monotonic_denotation S (L.wand e1 e2) := by
-  intro m n Hmn
-  simp [W.interp_wand]
-  intro H m0 m1 Hm0m1 Hi1
-  apply H
-  · exact Kripke.Structure.kle_trans n m m0 Hmn Hm0m1
-  apply Hi1
-
-theorem Mono.base [Kripke.Structure M] (S : Kripke.Semantics M B) [Mod : Kripke.Model M B] :
-    Kripke.monotonic_denotation S (L.base b) := by
-  unfold Kripke.monotonic_denotation
-  intro m n Hnm
-  simp [Kripke.Semantics.interp_base]
-  intro H1
-  apply Mod.kle_ainterp_mono
-  · apply Hnm
-  · apply H1
-
-theorem Mono.bot [Kripke.Structure M] (S : Kripke.Semantics M B) :
-    Kripke.monotonic_denotation S L.bot := by
-  unfold Kripke.monotonic_denotation
-  simp [Kripke.Semantics.interp_bot]
-
-theorem Mono.and [Kripke.Structure M] (S : Kripke.Semantics M B) :
-    Kripke.monotonic_denotation S φ ->
-    Kripke.monotonic_denotation S ψ ->
-    Kripke.monotonic_denotation S (L.and φ ψ) := by
-  unfold Kripke.monotonic_denotation
-  simp [Kripke.Semantics.interp_and]
-  intro Hm1 Hm2 m n Hnm Hφ Hψ
-  apply And.intro
-  · apply (Hm1 _ _ Hnm)
-    trivial
-  · apply (Hm2 _ _ Hnm)
-    trivial
-
-theorem Mono.or [Kripke.Structure M] (S : Kripke.Semantics M B) :
-    Kripke.monotonic_denotation S φ ->
-    Kripke.monotonic_denotation S ψ ->
-    Kripke.monotonic_denotation S (L.or φ ψ) := by
-  unfold Kripke.monotonic_denotation
-  simp [Kripke.Semantics.interp_or]
-  intro Hm1 Hm2 m n Hnm H
-  cases H
-  · left
-    apply (Hm1 _ _ Hnm)
-    trivial
-  · right
-    apply (Hm2 _ _ Hnm)
-    trivial
-
-theorem Mono.imp [Kripke.Structure M] (S : Kripke.Semantics M B) :
-    Kripke.monotonic_denotation S (L.imp φ ψ) := by
-  unfold Kripke.monotonic_denotation
-  simp [Kripke.Semantics.interp_imp]
-  intro m n Hmn H m1 Hm1 H2
-  apply H
-  · exact Kripke.Structure.kle_trans n m m1 Hmn Hm1
-  trivial
-
-theorem Mono.emp_dcsa [Kripke.Structure M] [SepC M] (S : Kripke.Semantics M B) [Kripke.EmpSemantics M B S] [DCSA M] :
-    Kripke.monotonic_denotation S L.emp := by
-  unfold Kripke.monotonic_denotation
-  simp [Kripke.EmpSemantics.interp_emp]
-  intro m n Hnm
-  simp [is_increasing]
-  intro h1 m2
-  rcases (DCSA.dcsa m m2 (m ∗ m2) n m2 (by rfl) Hnm (Kripke.Structure.kle_refl m2)) with ⟨ n', Hn', H'n' ⟩
-  apply Kripke.Structure.kle_trans _ _ _ _ H'n'
-  rw [<- Hn']
-  apply h1
-
+/-
 -- TODO: Lemma 1: make conversion instances for StrongWand and WeakWand in a UCSA, resp. DCSA
 
 -- TODO: In upwards and downwards closed model, all programs in the flat semantics have monotonic denotation
 
 -- TODO: Semantic equivalence lemmas
-
-/-
-Residue and unitality
 -/
-
-/--
-m is a residue of m
--/
-def residue [Kripke.Ord M] [SepC M] (m n : M) : Prop :=
-  ∃ n', m ∗ n' = n ∧ n << n'
-
-/--
-All elements have an increasing residue
--/
-class Unital (M : Type) [Kripke.Ord M] [SepC M] where
-  unital : ∀ m, ∃ unit : M, residue unit m ∧ is_increasing unit
-
-/-
-Soundness of IP rules against in a model that is upwards closed, downwards closed, and unital
--/
-
--- FIXME: Changed to packed class
-class SoundIPModel (M : Type) [Kripke.Ord M] where
-  inst_sepC : SepC M
-  inst_SA : SA M
-  inst_ucsa : UCSA M
-  inst_dcsa : DCSA M
-  inst_unital : Unital M
-
-instance SoundIPModel_SepC [Kripke.Ord M] [I : SoundIPModel M] : SepC M := by cases I; trivial
-
-instance SoundIPModel_DCSA [Kripke.Ord M] [I : SoundIPModel M] : DCSA M := by cases I; trivial
-
-instance SoundIPModel_UCSA [Kripke.Ord M] [I : SoundIPModel M] : UCSA M := by cases I; trivial
-
-instance SoundIPModel_SA [Kripke.Ord M] [I : SoundIPModel M] : SA M := by cases I; trivial
-
-instance SoundIPModel_Unital [Kripke.Ord M] [I : SoundIPModel M] : Unital M := by cases I; trivial
-
-
-
-class FlatSemantics (M B : Type) [Kripke.Ord M] [SepC M] (S : Kripke.Semantics M B) where
-   inst_EmpSemantics : Kripke.EmpSemantics M B S
-   inst_WeakWandSemantics : Kripke.WeakWandSemantics M B S
-   inst_WeakSepSemantics : Kripke.WeakSepSemantics M B S
-
-instance FlatSemantics_EmpSemantics (M B : Type) [Kripke.Ord M] [SepC M] (S : Kripke.Semantics M B) [I : FlatSemantics M B S] :
-    Kripke.EmpSemantics M B S := by
-  cases I; trivial
-
-instance FlatSemantics_WeakWandSemantics (M B : Type) [Kripke.Ord M] [SepC M] (S : Kripke.Semantics M B) [I : FlatSemantics M B S] :
-    Kripke.WeakWandSemantics M B S := by
-  cases I; trivial
-
-instance FlatSemantics_WeakSepSemantics (M B : Type) [Kripke.Ord M] [SepC M] (S : Kripke.Semantics M B) [I : FlatSemantics M B S] :
-    Kripke.WeakSepSemantics M B S := by
-  cases I; trivial
-
-/--
-Monotonicity for the weak semantics
--/
-theorem SoundIPModel.mono (M B : Type) [Kripke.Structure M] (S : Kripke.Semantics M B) [Kripke.Model M B]
-        [SoundIPModel M] [FlatSemantics M B S] :
-    ∀ e, Kripke.monotonic_denotation S e := by
-  intro e
-  induction e
-  · apply Mono.base
-  · apply Mono.bot
-  · apply Mono.and <;> trivial
-  · apply Mono.or <;> trivial
-  · apply Mono.imp
-  · apply Mono.emp_dcsa
-  · apply Mono.weak_sep <;> trivial
-  · apply Mono.weak_wand <;> trivial
-
-theorem Soundness.imp1 {φ ψ : L B}
-    [Kripke.Structure M] (S : Kripke.Semantics M B) [Kripke.Model M B] [SoundIPModel M] [FlatSemantics M B S] :
-    ∀ m : M, S.interp m <| imp φ <| imp ψ φ := by
-  intro m
-  rw [Kripke.Semantics.interp_imp]
-  intro m0 _ Hφ
-  rw [Kripke.Semantics.interp_imp]
-  intro m1 Hm1 _
-  apply SoundIPModel.mono
-  · apply Hm1
-  apply Hφ
-
-theorem Soundness.imp2 {φ ψ : L B}
-    [Kripke.Structure M] (S : Kripke.Semantics M B) [Kripke.Model M B] [SoundIPModel M] [FlatSemantics M B S] :
-    ∀ m : M, S.interp m <| imp (imp φ (imp ψ χ)) <| imp (imp φ ψ) <| imp φ χ := by
-  intro m
-  simp [Kripke.Semantics.interp_imp]
-  intro m1 _ H m2 Hm2 H3 m4 Hm4 Hm4φ
-  apply (H _ ?G1 Hm4φ m4 ?G2)
-  case G1 => exact Kripke.Structure.kle_trans m1 m2 m4 Hm2 Hm4
-  case G2 => exact Kripke.Structure.kle_refl m4
-  apply (H3 _ Hm4 Hm4φ)
-
-theorem Soundness.andI {φ ψ : L B}
-    [Kripke.Structure M] (S : Kripke.Semantics M B) [Kripke.Model M B] [SoundIPModel M] [FlatSemantics M B S] :
-    ∀ m : M, S.interp m <| imp φ <| imp ψ (and φ ψ) := by
-  simp [Kripke.Semantics.interp_imp, Kripke.Semantics.interp_and]
-  intro m0 m1 _ Hφ m3 Hm1m3 Hψ
-  apply And.intro
-  · apply SoundIPModel.mono _ _ _ _ _ _ Hm1m3
-    trivial
-  · trivial
-
-theorem Soundness.andE1 {φ ψ : L B}
-    [Kripke.Structure M] (S : Kripke.Semantics M B) [Kripke.Model M B] [SoundIPModel M] [FlatSemantics M B S] :
-    ∀ m : M, S.interp m <| imp (and φ ψ) φ := by
-  simp [Kripke.Semantics.interp_imp, Kripke.Semantics.interp_and]
-  intros
-  trivial
-
-theorem Soundness.andE2 {φ ψ : L B}
-    [Kripke.Structure M] (S : Kripke.Semantics M B) [Kripke.Model M B] [SoundIPModel M] [FlatSemantics M B S] :
-    ∀ m : M, S.interp m <| imp (and φ ψ) ψ := by
-  simp [Kripke.Semantics.interp_imp, Kripke.Semantics.interp_and]
-
-theorem Soundness.orI1 {φ ψ : L B}
-    [Kripke.Structure M] (S : Kripke.Semantics M B) [Kripke.Model M B] [SoundIPModel M] [FlatSemantics M B S] :
-    ∀ m : M, S.interp m <| imp φ (or φ ψ) := by
-  simp [Kripke.Semantics.interp_imp, Kripke.Semantics.interp_or]
-  intros
-  left
-  trivial
-
-theorem Soundness.orI2 {φ ψ : L B}
-    [Kripke.Structure M] (S : Kripke.Semantics M B) [Kripke.Model M B] [SoundIPModel M] [FlatSemantics M B S] :
-    ∀ m : M, S.interp m <| imp ψ (or φ ψ) := by
-  simp [Kripke.Semantics.interp_imp, Kripke.Semantics.interp_or]
-  intros
-  right
-  trivial
-
-theorem Soundness.orE {φ ψ : L B}
-    [Kripke.Structure M] (S : Kripke.Semantics M B) [Kripke.Model M B] [SoundIPModel M] [FlatSemantics M B S] :
-    ∀ m : M, S.interp m <| imp (imp φ χ) <| imp (imp ψ χ) <| imp (or φ ψ) χ := by
-  simp [Kripke.Semantics.interp_imp, Kripke.Semantics.interp_or]
-  intro m0 m1 _ H1 m2 m1m2 H2 m3 m2m3 H3
-  cases H3
-  · apply H1
-    · exact Kripke.Structure.kle_trans m1 m2 m3 m1m2 m2m3
-    · trivial
-  · apply H2
-    · exact m2m3
-    · trivial
-
-theorem Soundness.botE {φ : L B}
-    [Kripke.Structure M] (S : Kripke.Semantics M B) [Kripke.Model M B] [SoundIPModel M] [FlatSemantics M B S] :
-    ∀ m : M, S.interp m <| imp bot φ := by
-  simp [Kripke.Semantics.interp_imp, Kripke.Semantics.interp_bot]
-
--- In this one, should m be the same in each? Or should it increase?
-theorem Soundness.mp {φ ψ : L B}
-    [Kripke.Structure M] (S : Kripke.Semantics M B) [Kripke.Model M B] [SoundIPModel M] [FlatSemantics M B S] :
-    ∀ m : M, S.interp m φ -> S.interp m (imp φ ψ) -> S.interp m ψ := by
-  simp [Kripke.Semantics.interp_imp]
-  intro m Hφ H
-  apply H
-  · exact Kripke.Structure.kle_refl m
-  · trivial
-
-/-
-Soundness for the SL axioms
--/
-theorem Soundness.scomm {φ : L B}
-    [Kripke.Structure M] (S : Kripke.Semantics M B) [Kripke.Model M B] [SoundIPModel M] [FlatSemantics M B S] [SA M] :
-    ∀ m : M, S.interp m <| imp (sep φ ψ) (sep ψ φ) := by
-  simp [Kripke.Semantics.interp_imp]
-  intro m0 m1 _
-  simp [Kripke.WeakSepSemantics.interp_sep]
-  intro m2 m3 m2m3 Hφ Hψ
-  exists m3
-  exists m2
-  apply And.intro
-  · rw [SA.sepC_comm]
-    trivial
-  apply And.intro
-  · trivial
-  · trivial
-
-theorem Soundness.sA1 {φ : L B}
-    [Kripke.Structure M] (S : Kripke.Semantics M B) [Kripke.Model M B] [SoundIPModel M] [FlatSemantics M B S] [SA M] :
-    (∀ m : M, (S.interp m <| imp (sep φ ψ) χ)) -> (∀ m : M, (S.interp m <| imp φ (wand ψ χ))) := by
-  simp [Kripke.Semantics.interp_imp, Kripke.WeakSepSemantics.interp_sep, Kripke.WeakWandSemantics.interp_wand]
-  intro H m1 m2 _ Hφ m3 Hψ
-  apply H (m2 ∗ m3) (m2 ∗ m3) (Kripke.Structure.kle_refl (m2 ∗ m3)) m2 m3 (by rfl) Hφ Hψ
-
-theorem Soundness.sA2 {φ : L B}
-    [Kripke.Structure M] (S : Kripke.Semantics M B) [Kripke.Model M B] [SoundIPModel M] [FlatSemantics M B S] [SA M] :
-    (∀ m : M, (S.interp m <| imp φ (wand ψ χ))) -> (∀ m : M, S.interp m <| imp (sep φ ψ) χ) := by
-  simp [Kripke.Semantics.interp_imp, Kripke.WeakSepSemantics.interp_sep, Kripke.WeakWandSemantics.interp_wand]
-  intro H m1 m2 m0m1 m3 m4 m3m42 Hφ Hψ
-  subst m3m42
-  apply H m3 m3 (Kripke.Structure.kle_refl m3) Hφ m4 Hψ
-
-theorem Soundness.semp {φ : L B}
-    [Kripke.Structure M] (S : Kripke.Semantics M B) [Kripke.Model M B] [SoundIPModel M] [FlatSemantics M B S] [SA M] :
-    ∀ m : M, S.interp m <| iff (sep φ emp) φ := by
-  unfold L.iff
-  simp [Kripke.Semantics.interp_and, Kripke.Semantics.interp_imp, Kripke.WeakSepSemantics.interp_sep, Kripke.EmpSemantics.interp_emp]
-  intro m0
-  apply And.intro
-  · intro m1 _ m2 m3 m231 Hφ HI
-    apply SoundIPModel.mono _ _ _ _ _ m2 ?G2 ?G3
-    · apply HI
-      rw [SA.sepC_comm]
-      trivial
-    · trivial
-  · intro m1 _ Hφ
-    rcases (Unital.unital m1) with ⟨ m1u, ⟨ m1r, Em1, Hm1r ⟩, Hu ⟩
-    exists m1r
-    exists m1u
-    apply And.intro
-    · rw [SA.sepC_comm]
-      trivial
-    apply And.intro
-    · apply SoundIPModel.mono _ _ _ _ _ m1 Hm1r Hφ
-    · trivial
-
-theorem Soundness.sassoc {φ : L B}
-    [Kripke.Structure M] (S : Kripke.Semantics M B) [Kripke.Model M B] [SoundIPModel M] [FlatSemantics M B S] [SA M] :
-    ∀ m : M, S.interp m <| imp (sep (sep φ ψ) χ) <| (sep φ (sep ψ χ)) := by
-  simp [Kripke.Semantics.interp_imp, Kripke.WeakSepSemantics.interp_sep]
-  intro m0 m1 m0m1 m2 m3 m231 m4 m5 m452
-  subst m231
-  subst m452
-  intro Hφ Hψ Hχ
-  exists m4
-  exists (m5 ∗ m3)
-  apply And.intro
-  · apply Eq.symm (SA.sepC_assoc m4 m5 m3)
-  apply And.intro
-  · trivial
-  exists m5
-  exists m3
-
-theorem Soundness.smono
-    [Kripke.Structure M] (S : Kripke.Semantics M B) [Kripke.Model M B] [SoundIPModel M] [FlatSemantics M B S] [SA M] :
-    (∀ m : M, (S.interp m <| imp φ1 ψ1)) -> (∀ m : M, S.interp m <| imp φ2 ψ2) -> (∀ m : M, S.interp m <| imp (sep φ1 φ2) (sep ψ1 ψ2)) := by
-  simp [Kripke.Semantics.interp_imp, Kripke.WeakSepSemantics.interp_sep]
-  intro H1 H2 m0 m1 m01 m2 m3 m231 Hp1 Hp2
-  subst m231
-  exists m2
-  exists m3
-  apply And.intro
-  · rfl
-  apply And.intro
-  · apply H1 m2 m2 (Kripke.Structure.kle_refl m2) Hp1
-  · apply H2 m3 m3 (Kripke.Structure.kle_refl m3) Hp2
-
-/-
-Soundness for the extensions
--/
-
-
-
-/-
-Soundness for the basic IP+SL system (removed base props)
--/
-
-inductive IPSL_deriv {B : Type} : L B -> Prop
-| mp     : IPSL_deriv φ -> IPSL_deriv (imp φ ψ) -> IPSL_deriv ψ
-| imp1   : IPSL_deriv <| imp φ <| imp ψ φ
-| imp2   : IPSL_deriv <| imp (imp φ (imp ψ χ)) <| imp (imp φ ψ) <| imp φ χ
-| andI   : IPSL_deriv <| imp φ <| imp ψ (and φ ψ)
-| andE1  : IPSL_deriv <| imp (and φ ψ) φ
-| andE2  : IPSL_deriv <| imp (and φ ψ) ψ
-| orI1   : IPSL_deriv <| imp φ (or φ ψ)
-| orI2   : IPSL_deriv <| imp ψ (or φ ψ)
-| orE    : IPSL_deriv <| imp (imp φ χ) <| imp (imp ψ χ) <| imp (or φ ψ) χ
-| botE   : IPSL_deriv <| imp bot φ
-| scomm  : IPSL_deriv <| imp (sep φ ψ) (sep ψ φ)
-| sA1    : IPSL_deriv (imp (sep φ ψ) χ) -> IPSL_deriv (imp φ (wand ψ χ))
-| sA2    : IPSL_deriv (imp φ (wand ψ χ)) -> IPSL_deriv (imp (sep φ ψ) χ)
-| semp   : IPSL_deriv (iff (sep φ emp) φ)
-| sassoc : IPSL_deriv (imp (sep (sep φ ψ) χ) <| (sep φ (sep ψ χ)))
-| smono  : IPSL_deriv (imp φ1 ψ1) -> IPSL_deriv (imp φ2 ψ2) -> IPSL_deriv (imp (sep φ1 φ2) (sep ψ1 ψ2))
-
-instance ISPL_deriv_IP_inst {B} : IP (@IPSL_deriv B) where
-mp     := IPSL_deriv.mp
-imp1   := IPSL_deriv.imp1
-imp2   := IPSL_deriv.imp2
-andI   := IPSL_deriv.andI
-andE1  := IPSL_deriv.andE1
-andE2  := IPSL_deriv.andE2
-orI1   := IPSL_deriv.orI1
-orI2   := IPSL_deriv.orI2
-orE    := IPSL_deriv.orE
-botE   := IPSL_deriv.botE
-
-instance ISPL_deriv_SL_inst {B} : SL (@IPSL_deriv B) where
-scomm  := IPSL_deriv.scomm
-sA1    := IPSL_deriv.sA1
-sA2    := IPSL_deriv.sA2
-semp   := IPSL_deriv.semp
-sassoc := IPSL_deriv.sassoc
-smono  := IPSL_deriv.smono
-
-
-theorem IPSL_kripke_soundness {B : Type} [Kripke.Structure M] (S : Kripke.Semantics M B) [Kripke.Model M B] [SoundIPModel M] [FlatSemantics M B S] :
-    ∀ φ : L B, IPSL_deriv φ -> ∀ m, S.interp m φ := by
-  intro φ H
-  induction H
-  · rename_i _ _ _ _ IH1 IH2
-    intro m
-    apply Soundness.mp
-    · apply IH1
-    · apply IH2
-  · apply Soundness.imp1
-  · apply Soundness.imp2
-  · apply Soundness.andI
-  · apply Soundness.andE1
-  · apply Soundness.andE2
-  · apply Soundness.orI1
-  · apply Soundness.orI2
-  · apply Soundness.orE
-  · apply Soundness.botE
-  · apply Soundness.scomm
-  · apply Soundness.sA1
-    trivial
-  · apply Soundness.sA2
-    trivial
-  · apply Soundness.semp
-  · apply Soundness.sassoc
-  · apply Soundness.smono
-    · trivial
-    · trivial
-
-
-
-
-
-
-section sound_model
-
--- Now if we can exhibit _some_ Kripke model with the above requirements, to prove the IPSL system is sound
-
-instance discrete_order {T : Type} : Kripke.Ord T where
-  kle := Eq
-
-instance discrete_structure {T : Type} : Kripke.Structure T where
-  kle_refl _ := by rfl
-  kle_trans := by
-    unfold Kripke.Ord.kle
-    unfold discrete_order
-    simp
-
-instance discrete_triv_ainterp {T1 T2: Type} : Kripke.AtomicInterp T1 T2 where
-  ainterp _ _ := True
-
-instance sepC_unit : SepC Unit where
-  sepC _ _ := PUnit.unit
-
--- #check
-instance discrete_model {T : Type} : Kripke.Model T Unit  where
-  kle_ainterp_mono _ _ _ H _ := by rw [<- H]; trivial
-
-instance unit_SA : SA Unit where
-  sepC_assoc := by simp
-  sepC_comm  := by simp
-
-instance unit_UCSA : UCSA Unit where
-  ucsa := by simp [Kripke.Ord.kle]
-
-instance unit_DCSA : DCSA Unit where
-  dcsa := by simp [Kripke.Ord.kle]
-
-instance unit_Unital : Unital Unit where
-  unital := by simp [residue, is_increasing, Kripke.Ord.kle]
-
-instance unit_SoundIPModel : SoundIPModel Unit where
-  inst_sepC := sepC_unit
-  inst_SA := unit_SA
-  inst_ucsa := unit_UCSA
-  inst_dcsa := unit_DCSA
-  inst_unital := unit_Unital
-
-
-def UnitSemantics : Kripke.Semantics Unit Unit := (@flat_semantics Unit Unit _ _ _)
-
-instance unit_empSemantics : Kripke.EmpSemantics Unit Unit UnitSemantics where
-  interp_emp := by simp [Kripke.Semantics.interp, UnitSemantics, flat_semantics]
-
-instance unit_weakWand : Kripke.WeakWandSemantics Unit Unit UnitSemantics where
-  interp_wand := by simp [Kripke.Semantics.interp, UnitSemantics, flat_semantics]
-
-instance unit_weakSep : Kripke.WeakSepSemantics Unit Unit UnitSemantics where
-  interp_sep := by simp [Kripke.Semantics.interp, UnitSemantics, flat_semantics]
-
-instance unit_flatSemantics : FlatSemantics Unit _ UnitSemantics where
-  inst_EmpSemantics := unit_empSemantics
-  inst_WeakWandSemantics := unit_weakWand
-  inst_WeakSepSemantics := unit_weakSep
-
-theorem IPSL_unit_soundness : @IPSL_deriv Unit bot -> False := by
-  intro K
-  have X := @IPSL_kripke_soundness Unit Unit _ UnitSemantics discrete_model unit_SoundIPModel _ bot K PUnit.unit
-  simp [Kripke.Semantics.interp, UnitSemantics, flat_semantics] at X
-
-end sound_model
