Order/Lib.lean
@@ -1,0 +1,7 @@
+/-- A reflexive relation -/
+class Reflexive (op : α → α → Prop) : Prop where
+  refl : {a : α} → op a a
+
+/-- A reflexive relation -/
+class Transitive (op : α → α → Prop) : Prop where
+  trans : {a b c : α} → op a b -> op b c -> op a c
